attempt to prove constant-timeness with stack allocation. fails - semantics need to be changed.

bedrock2/src/bedrock2Examples/stackalloc.v
@@ -18,7 +18,7 @@ Definition stackdisj := func! () ~> (a,b) {
   /*skip*/
 }.
 
-Require bedrock2.WeakestPrecondition.
+Require Import bedrock2.WeakestPrecondition.
 Require Import bedrock2.Semantics bedrock2.FE310CSemantics.
 Require Import coqutil.Map.Interface bedrock2.Map.Separation bedrock2.Map.SeparationLogic.
 
@@ -54,8 +54,99 @@ Section WithParameters.
     end end end.
 
     intuition congruence.
-  Qed.
+  Qed. Locate "ctfunc _".
 
+  Instance ct_spec_of_stacknondet : ct_spec_of "stacknondet" :=
+    ctfunc! "stacknondet" | / (dummy3 : nat) | (dummy4 : nat),
+      { requires tr mem := True }.
+
+  Definition stackall := func! () ~> () {
+  stackalloc 4 as a;
+  x = load4(a)
+                           }.
+
+  Instance ct_spec_of_stackall : ct_spec_of "stackall" :=
+    ctfunc! "stackall" | / (dummy3 : nat) | (dummy4 : nat),
+      { requires tr mem := True }.
+
+  Lemma stackall_ct : program_logic_ct_goal_for_function! stackall.
+  Proof.
+    straightline. straightline. straightline. straightline. straightline. straightline.
+    straightline. straightline. straightline. straightline.
+    set (R := eq mem0).
+    pose proof (eq_refl : R mem0) as Hmem0.
+    straightline_stackalloc. eexists. eexists. split.
+    { repeat straightline. eexists. split; repeat straightline. Print ptsto.
+      repeat (destruct stack as [|?b stack]; try solve [cbn in H2; Lia.lia]; []).
+      clear H2. seprewrite_in_by @scalar32_of_bytes Hmem0 reflexivity.
+      repeat straightline. }
+    repeat straightline. trace_alignment. Unshelve.
+    2: { Abort.
+  (*Abort.
+    instantiate (1 := [Semantics.read access_size.four a]%list).
+
+    eexists. eexists. split.
+    { repeat straightline. Search load. Search anybytes. Print Lift1Prop.impl1.
+      match goal with Hanybytes: Memory.anybytes ?a ?n ?mStack |- _ =>
+  let m := match goal with H : map.split ?mCobined ?m mStack |- _ => m end in
+  let mCombined := match goal with H : map.split ?mCobined ?m mStack |- _ => mCobined end in
+  let Hsplit := match goal with H : map.split ?mCobined ?m mStack |- _ => H end in
+  let Hm := multimatch goal with H : _ m |- _ => H end in
+  let Hm' := fresh Hm in
+  let Htmp := fresh in
+  let Pm := match type of Hm with ?P m => P end in idtac end.
+  assert_fails (assert (Separation.sep Pm (Array.array Separation.ptsto (Interface.word.of_Z (BinNums.Zpos BinNums.xH)) a _) mCombined) as _ by ecancel_assumption) end.
+  rename Hm into Hm';
+  let stack := fresh "stack" in
+  let stack_length := fresh "length_" stack in (* MUST remain in context for deallocation *)
+  destruct (Array.anybytes_to_array_1 mStack a n Hanybytes) as (stack&Htmp&stack_length);
+  epose proof (ex_intro _ m (ex_intro _ mStack (conj Hsplit (conj Hm' Htmp)))
+  : Separation.sep _ (Array.array Separation.ptsto (Interface.word.of_Z (BinNums.Zpos BinNums.xH)) a _) mCombined) as Hm;
+  clear Htmp; (* note: we could clear more here if we assumed only one separation-logic description of each memory is present *)
+  try (let m' := fresh m in rename m into m'); rename mCombined into m;
+  ( assert (BinInt.Z.of_nat (Datatypes.length stack) = n)
+  by (rewrite stack_length; apply (ZifyInst.of_nat_to_nat_eq n))
+  || fail 2 "negative stackalloc of size" n )
+  end. eapply anybytes_to_scalar in H0. Print scalar. exists. veauto. }
+    { split. { eauto. } simpl. Print trace_alignment. symmetry. eapply List.app_nil_l. }
+  Qed. try straightline. straightline_stackalloc.*)
+
+  Lemma stacknondet_ct : program_logic_ct_goal_for_function! stacknondet.
+  Proof.
+    straightline. straightline. straightline. straightline. straightline. straightline.
+    straightline. straightline. straightline. straightline. straightline.
+    repeat straightline.
+    set (R := eq mem0).
+    pose proof (eq_refl : R mem0) as Hmem0.
+    repeat straightline.
+    repeat (destruct stack as [|?b stack]; try solve [cbn in H2; Lia.lia]; []);
+      clear H H0 H1 length_stack.
+    seprewrite_in_by @scalar32_of_bytes Hmem0 reflexivity.
+    repeat straightline.
+    Import symmetry eplace.
+    seprewrite_in_by (symmetry! @scalar32_of_bytes) Hmem0 reflexivity.
+    cbn [Array.array] in Hmem0.
+    Import Ring_tac.
+    repeat straightline.
+    assert ((Array.array ptsto (word.of_Z 1) a [(Byte.byte.of_Z (word.unsigned v0)); b0; b1; b2] ⋆ R)%sep m).
+    { cbn [Array.array].
+      use_sep_assumption; cancel; Morphisms.f_equiv; f_equal; f_equal; ring. }
+    seprewrite_in_by @scalar32_of_bytes H0 reflexivity.
+    repeat straightline.
+    seprewrite_in_by (symmetry! @scalar32_of_bytes) H0 reflexivity.
+    repeat straightline.
+    Tactics.ssplit; eauto.
+    eexists. eexists. Print anybytes. split; try split; try straightline.
+
+    subst v. subst v1. subst ss.
+    eapply Properties.word.unsigned_inj.
+    rewrite ?Properties.word.unsigned_sru_nowrap.
+    2,3: rewrite ?Properties.word.unsigned_of_Z_nowrap by Lia.lia; reflexivity.
+    rewrite ?Properties.word.unsigned_of_Z_nowrap; try Lia.lia.
+    2,3: eapply (LittleEndianList.le_combine_bound [_;_;_;_]).*)
+  (*eexists. eexists. split; repeat straightline.
+    { eexists. split; repeat straightline. Search anybytes. all: cbv [anybytes] in H0.
+      1: straightline. 1: straightline.*) Abort.
   Instance spec_of_stacknondet : spec_of "stacknondet" := fun functions => forall m t,
       WeakestPrecondition.call functions
         "stacknondet" t m [] (fun t' m' rets => exists a b, rets = [a;b] /\ a = b /\ m'=m/\(filterio t')=(filterio t)).
